Checkpoint, almost building... Failure at Extract.v due to missing components in modules. E.g., MEM and MEMORY_THEORY in Lang are just declared, but not filled in.

src/coq/Handlers/MemoryModel.v
@@ -1,5 +1,6 @@
 From Vellvm.Syntax Require Import
-     DataLayout.
+     DataLayout
+     DynamicTypes.
 
 From Vellvm.Semantics Require Import
      MemoryParams
@@ -27,19 +28,13 @@ From Coq Require Import
 
 Import Basics.Basics.Monads.
 
-Require Import Vellvm.Semantics.MemoryAddress.
-Require Import Vellvm.Syntax.DynamicTypes.
-Require Import Vellvm.Semantics.DynamicValues.
-Require Import Vellvm.Semantics.Memory.Sizeof.
+(* Module types for memory models to allow different memory models to be plugged in. *)
+Module Type MemoryModel (LP : LLVMParams) (MP : MemoryParams LP).
+  Import LP.Events.
+  Import LP.ADDR.
 
-Module Type MemoryState (Addr:MemoryAddress.ADDRESS) (IP : INTPTR) (SIZEOF : Sizeof) (PROV : PROVENANCE Addr) (Events : LLVM_INTERACTIONS Addr IP SIZEOF).
-  Import PROV.
-  Import Addr.
-  Import Events.DV.
-
-  Import MonadNotation.
-  Open Scope monad.
-
+  (* TODO: Clean up / move this stuff *)
+  Import LP.PROV.
   Parameter store_id : Type.
 
   Class MonadProvenance (M : Type -> Type) : Type :=
@@ -55,77 +50,13 @@ Module Type MemoryState (Addr:MemoryAddress.ADDRESS) (IP : INTPTR) (SIZEOF : Siz
       put_mem_state : MemState -> M unit
     }.
 
-  Definition fresh_allocation_id {M} `{Monad M} `{MonadProvenance M} : M AllocationId
-    := prov <- fresh_provenance;;
-       ret (provenance_to_allocation_id prov).
 
-  (* Datatype for the state of memory *)
-  Parameter MemState : Type.
-  Parameter initial_memory_state : MemState.
-
-  Parameter allocate :
-    forall {M}
-      `{Monad M}
-      `{MonadMemState MemState}
-      `{MonadProvenance M} `{MonadStoreID M}
-      `{RAISE_ERROR M} `{RAISE_UB M} `{RAISE_OOM M},
-      dtyp -> M addr.
-
-  Parameter allocated :
-    forall {M}
-      `{Monad M}
-      `{MonadMemState MemState}
-      (ptr : addr),
-      M bool.
-
-  Parameter read :
-    forall (mem : MemState) (ptr : addr) (t : dtyp), err uvalue.
-
-  Parameter write :
-    forall {M}
-      `{MonadState MemState}
-      `{MonadStoreID M}
-      `{RAISE_ERROR M} `{RAISE_UB M} `{RAISE_OOM M}
-      (ptr : addr) (v : uvalue) (t : dtyp),
-      M unit.
-
-  Import SIZEOF.
-
-  Record ext_memory (m1 : MemState) (a : addr) (τ : dtyp) (v : uvalue) (m2 : MemState) : Prop :=
-    {
-      (* TODO: might want to extend this so if the size is 0 I know
-               what the value of read is... *)
-      new_lu  : sizeof_dtyp τ <> 0%N -> read m2 a τ = inr v;
-      old_lu  : forall a' τ', allocated a' m1 ->
-                         no_overlap_dtyp a τ a' τ' ->
-                         read m2 a' τ' = read m1 a' τ'
+  Class MemMonad (MemState : Type) (M : Type -> Type)
+        `{MonadProvenance M} `{MonadStoreID M} `{MonadMemState MemState M}
+        `{RAISE_ERROR M} `{RAISE_UB M} `{RAISE_OOM M} : Type
+    :=
+    { MemMonad_runs_to {A} (ma : M A) (ms : MemState) : option (MemState * A);
     }.
-
-    Definition same_reads (m1 m2 : memory_stack) : Prop := forall a τ, read m1 a τ = read m2 a τ.
-
-    Record allocate_spec (m1 : memory_stack) (τ : dtyp) (m2 : memory_stack) (a : addr) : Prop :=
-      {
-      was_fresh : ~ allocated a m1;
-      is_allocated : ext_memory m1 a τ (UVALUE_Undef τ) m2
-      }.
-
-    Record write_spec (m1 : memory_stack) (a : addr) (v : dvalue) (m2 : memory_stack) : Prop :=
-      {
-      was_allocated : allocated a m1;
-      is_written    : forall τ, is_supported τ ->
-                           dvalue_has_dtyp v τ ->
-                           ext_memory m1 a τ (dvalue_to_uvalue v) m2
-      }.
-
-    Record read_spec (m : memory_stack) (a : addr) (τ : dtyp) (v : uvalue) : Prop :=
-      {
-      is_read : read m a τ = inr v
-      }.
-End MemoryState.
-
-(* Module types for memory models to allow different memory models to be plugged in. *)
-Module Type MemoryModel (LP : LLVMParams) (MP : MemoryParams LP).
-  Import LP.Events.
 
   (* TODO: Should DataLayout be here? 
 
@@ -138,9 +69,33 @@ Module Type MemoryModel (LP : LLVMParams) (MP : MemoryParams LP).
    *)
   Parameter datalayout : DataLayout.
 
-  (* Datatype for the state of memory *)
+  (** Datatype for the state of memory *)
   Parameter MemState : Type.
   Parameter initial_memory_state : MemState.
+
+  (** Basic operations on the state of logical memory. *)
+  Parameter allocate :
+    forall {M : Type -> Type}
+      `{MemMonad MemState M},
+      dtyp -> M addr.
+
+  Parameter allocated :
+    forall {M : Type -> Type}
+      `{MemMonad MemState M}
+      (ptr : addr),
+      M bool.
+
+  Parameter read :
+    forall (mem : MemState) (ptr : addr) (t : dtyp), err uvalue.
+
+  Parameter write :
+    forall {M : Type -> Type}
+      `{MemMonad MemState M}
+      (ptr : addr) (v : uvalue) (t : dtyp),
+      M unit.
+
+  (** Operations for interacting with the concrete layout of memory. *)
+  Parameter reserve_block : MemState -> LP.IP.intptr -> N -> option MemState.
 
   (* TODO: Should we generalize this? *)
   Definition MemStateT := stateT MemState.
@@ -157,10 +112,4 @@ Module Type MemoryModel (LP : LLVMParams) (MP : MemoryParams LP).
       forall {E} `{FailureE -< E} `{PickE -< E} `{UBE -< E}, IntrinsicE ~> MemStateT (itree E).
    End Handlers.
 
-  (* For registering a physical address of a given size in memory
-
-     May fail if the block cannot be registered (likely because it
-     overlaps with non-free memory).
-   *)
-  Parameter reserve_block : MemState -> LP.IP.intptr -> N -> option MemState.
 End MemoryModel.
