src/coq/Handlers/MemoryState.v
@@ -1,0 +1,141 @@
+Require Import Vellvm.Syntax.DynamicTypes.
+
+From Vellvm.Semantics Require Import
+     LLVMParams
+     LLVMEvents
+     DynamicValues
+     MemoryParams
+     MemoryAddress
+     Memory.Sizeof
+     Memory.Overlaps.
+
+From Vellvm.Utils Require Import
+     Error.
+
+From ExtLib Require Import
+     Structures.Monads
+     Structures.Functor
+     Data.Monads.StateMonad.
+
+From Coq Require Import
+     ZArith.
+
+Module Type MemoryTypeSupport.
+  Parameter is_supported : dtyp -> Prop.
+End MemoryTypeSupport.
+
+Module Type MemoryState (LP : LLVMParams).
+  Import LP.PROV.
+  Import LP.ADDR.
+  Import LP.Events.DV.
+
+  Import MonadNotation.
+  Open Scope monad.
+
+  (* TODO: Clean up / move this stuff *)
+  Parameter store_id : Type.
+
+  Class MonadProvenance (M : Type -> Type) : Type :=
+    { fresh_provenance : M Provenance
+    }.
+
+  Class MonadStoreID (M : Type -> Type) : Type :=
+    { fresh_sid : M store_id
+    }.
+
+  Class MonadMemState (MemState : Type) (M : Type -> Type) : Type :=
+    { get_mem_state : M MemState;
+      put_mem_state : MemState -> M unit
+    }.
+
+  Definition fresh_allocation_id {M} `{Monad M} `{MonadProvenance M} : M AllocationId
+    := prov <- fresh_provenance;;
+       ret (provenance_to_allocation_id prov).
+
+  (** Datatype for the state of memory *)
+  Parameter MemState : Type.
+  Parameter initial_memory_state : MemState.
+
+  (** Basic operations on the state of memory. *)
+  Parameter allocate :
+    forall {M : Type -> Type}
+      `{Monad M}
+      `{MonadMemState MemState}
+      `{MonadProvenance M} `{MonadStoreID M}
+      `{RAISE_ERROR M} `{RAISE_UB M} `{RAISE_OOM M},
+      dtyp -> M addr.
+
+  Parameter allocated :
+    forall {M : Type -> Type}
+      `{Monad M}
+      `{MonadMemState MemState}
+      (ptr : addr),
+      M bool.
+
+  Parameter read :
+    forall (mem : MemState) (ptr : addr) (t : dtyp), err uvalue.
+
+  Parameter write :
+    forall {M : Type -> Type}
+      `{MonadState MemState}
+      `{MonadStoreID M}
+      `{RAISE_ERROR M} `{RAISE_UB M} `{RAISE_OOM M}
+      (ptr : addr) (v : uvalue) (t : dtyp),
+      M unit.
+
+End MemoryState.
+
+(** Lemmas, helper functions, and specifications relating to the state of memory. *)
+Module MemoryStateHelpers (LP : LLVMParams) (OVER : Overlaps LP.ADDR) (MS : MemoryState LP) (MTS : MemoryTypeSupport).
+  Import LP.PROV.
+  Import LP.ADDR.
+  Import LP.Events.DV.
+  Import MS.
+  Import MTS.
+
+  Module OVER_H := OverlapHelpers LP.ADDR LP.SIZEOF OVER.
+  Import OVER_H.
+  Import LP.SIZEOF.
+
+  Instance MonadState_MonadMemState {M} `{MonadState MemState M} : MonadMemState MemState M
+    := {
+      get_mem_state := get;
+      put_mem_state := put;
+    }.
+
+  (** Check if an address is allocated given the state of memory. *)
+  Definition addr_allocated (a : addr) (ms : MemState) : bool
+    := evalState (allocated a) ms.
+
+    (** Specification of memory state operations *)
+  Record ext_memory (m1 : MemState) (a : addr) (τ : dtyp) (v : uvalue) (m2 : MemState) : Prop :=
+    {
+      (* TODO: might want to extend this so if the size is 0 I know
+               what the value of read is... *)
+      new_lu  : sizeof_dtyp τ <> 0%N -> read m2 a τ = inr v;
+      old_lu  : forall a' τ', addr_allocated a' m1 = true ->
+                         no_overlap_dtyp a τ a' τ' = true ->
+                         read m2 a' τ' = read m1 a' τ'
+    }.
+
+  Definition same_reads (m1 m2 : MemState) : Prop := forall a τ, read m1 a τ = read m2 a τ.
+
+  Record allocate_spec (m1 : MemState) (τ : dtyp) (m2 : MemState) (a : addr) : Prop :=
+    {
+      was_fresh : addr_allocated a m1 = false;
+      is_allocated : ext_memory m1 a τ (UVALUE_Undef τ) m2
+    }.
+
+  Record write_spec (m1 : MemState) (a : addr) (v : dvalue) (m2 : MemState) : Prop :=
+    {
+      was_allocated : addr_allocated a m1 = true;
+      is_written    : forall τ, is_supported τ ->
+                           dvalue_has_dtyp v τ ->
+                           ext_memory m1 a τ (dvalue_to_uvalue v) m2
+    }.
+
+  Record read_spec (m : MemState) (a : addr) (τ : dtyp) (v : uvalue) : Prop :=
+    {
+      is_read : read m a τ = inr v
+    }.
+End MemoryStateHelpers.
