src/coq/Semantics/TopLevel.v
@@ -168,7 +168,7 @@ Module Type LLVMTopLevel (IS : InterpreterStack).
     'defns <- map_monad address_one_function (m_definitions mcfg) ;;
     'addr <- trigger (GlobalRead (Name entry)) ;;
     'rv <- denote_mcfg defns ret_typ (dvalue_to_uvalue addr) args ;;
-    trigger (pick rv True).
+    trigger (pick_uvalue True rv).
 
 
   (* main_args and denote_vellvm_main may not be needed anymore, but I'm keeping them 
